Updated for new names in pgcl src e.g. NondetAssign

examples/pgcl/examples/simpledcScript.sml
@@ -16,14 +16,15 @@
 (*
 app load
   ["bossLib","realLib","rich_listTheory","stringTheory",
-   "metisLib","posrealLib","expectationTheory","intLib", "wpTheory", "valueTheory", "arithmeticTheory"];
+   "metisLib","posrealLib","expectationTheory","intLib", "wpTheory", "valueTheory", "arithmeticTheory",
+   "stringLib", "looprulesTheory"];
 quietdec := true;
 *)
 
-open HolKernel Parse boolLib bossLib intLib realLib metisLib;
+open HolKernel Parse boolLib bossLib intLib realLib metisLib stringLib;
 open combinTheory listTheory rich_listTheory stringTheory integerTheory
      realTheory;
-open posetTheory posrealTheory posrealLib expectationTheory wpTheory valueTheory arithmeticTheory;
+open posetTheory posrealTheory posrealLib expectationTheory wpTheory valueTheory arithmeticTheory looprulesTheory;
 
 (*
 quietdec := false;
@@ -91,12 +92,20 @@ val No_def = Define `No = Int 0`;
 val initialize_var_N_def = Define
    `initialize_var_N n = Assign "N" (\s. Int (&n))`;
 
+val initialize_var_NSApays_def = Define
+   `initialize_var_NSApays nsapays = 
+	if nsapays then Assign "NSApays" (\s. Yes)
+	           else Assign "NSApays" (\s. No)`;
+
 val set_payer_def = Define
-  `set_payer n =
-	Demonchoice "payer" (zero_to_n_Int_list (SUC n))`;
+  `set_payer n nsapays =
+	if nsapays then Assign "payer" (\s. Int (&n))
+		   else NondetAssign "payer" (zero_to_n_Int_list n)`;
 
 val initialize_def = Define
-  `initialize n = Program [initialize_var_N n; set_payer n]`;
+  `initialize n nsapays = Program [initialize_var_N n; 
+                                   initialize_var_NSApays nsapays; 
+                                   set_payer n nsapays]`;
 
 val flip_coins_def = Define
    `flip_coins =
@@ -105,7 +114,7 @@ val flip_coins_def = Define
 	  New_Array "Coins" "N";
 	  For_0_to_n "i" "N"
 	   [
-	   	Probchoice "coinflip" [Heads; Tails];
+	   	ProbAssign "coinflip" [Heads; Tails];
 	   	Assign_Array_i "Coins" "i" (\s. s "coinflip")
 	   ]
 	]`;
@@ -132,10 +141,10 @@ val compute_result_def = Define
    `compute_result = Assign "result" (\s. Xor (s "Announces"))`;
 
 val dcprog_def = Define
-   `dcprog_def n =
+   `dcprog n nsapays =
 	Program
 	[
-	   initialize n;
+	   initialize n nsapays;
 	   flip_coins;
 	   set_announcements;
 	   compute_result
@@ -144,6 +153,8 @@ val dcprog_def = Define
 (* ------------------------------------------------------------------------- *)
 (* Proofs                                                                    *)
 (* ------------------------------------------------------------------------- *)
+
+(* ----------------- zero_to_n_Int_list proofs ----------------------------- *)
 
 val zero_to_n_Int_list_length = store_thm
   ("zero_to_n_Int_list_length",
@@ -245,6 +256,8 @@ val zero_to_n_Int_list_contains_Int = store_thm
 	 ++ METIS_TAC [])
    ++ METIS_TAC []);
 
+(* ------------------- initialize_var_N proofs ----------------------------- *)
+
 val initialize_var_N_term = store_thm
   ("initialize_var_N_term",
    ``!n. (wp (initialize_var_N n) One) = One``,
@@ -260,36 +273,78 @@ val initialize_var_N_result2 = store_thm
    ``!n. (wp (initialize_var_N n) (\s. if (s"N" = Int(&n)) then 1 else 0)) = One``,
    RW_TAC std_ss [initialize_var_N_def, wp_def, assign_def, One_def]);
 
+(* ------------------- initialize_var_NSApays proofs ----------------------- *)
+
+val initialize_var_NSApays_term = store_thm
+  ("initialize_var_NSApays_term",
+   ``!nsapays. (wp (initialize_var_NSApays nsapays) One) = One``,
+    RW_TAC std_ss [initialize_var_NSApays_def, wp_def, One_def]);
+
+val initialize_var_NSApays_result = store_thm
+  ("initialize_var_NSApays_result",
+   ``!nsapays. (wp (initialize_var_NSApays nsapays) 
+		   (\s. if nsapays then
+				(if (s "NSApays") = Yes then 1 else 0)
+			else
+				(if (s "NSApays") = No then 1 else 0))) = One``,
+   RW_TAC std_ss [initialize_var_NSApays_def, wp_def, assign_def, 
+                  Yes_def, No_def, One_def, num_of_value_def, 
+		  int_of_value_def, NUM_OF_INT]);
+
+(* ------------------------- general arithmetic proof ---------------------- *)
+
+val LESS_EQ_EQ_LESS_SUC = store_thm
+  ("LESS_EQ_EQ_LESS_SUC",
+   ``!n m. (n <= m) = (n < SUC m)``,
+   RW_TAC arith_ss []);
+
+val posreal_of_SUC = store_thm
+  ("posreal_of_SUC",
+   ``(&(SUC n)) = (& n) + (1:posreal)``,
+   RW_TAC posreal_ss [posreal_of_num_inj]);
+
+val subr1_inv_eq_zero = store_thm
+  ("subr1_inv_eq_zero",
+   ``!x. (1 - inv x = 0) = (x < 1 \/ (x = 1))``,
+   `!x. ((x < 1) \/ (inv x = 1)) ==> (1 - inv x = 0)`
+	by (RW_TAC posreal_ss []
+	    >> (SPOSE_NOT_THEN STRIP_ASSUME_TAC
+	    	++ `~(1 - inv x <= 0)` by RW_TAC posreal_ss [le_zero]
+	    	++ `~(1=infty)` by RW_TAC posreal_ss []
+	    	++ `~(1 <= 0 + inv x)` by METIS_TAC [sub_le_eq]
+	    	++  FULL_SIMP_TAC std_ss [add_lzero, inv_one_le]
+	   	 ++ METIS_TAC [le_total, preal_lt_def])
+	    ++ RW_TAC posreal_ss [])
+   ++ `!x. (1 - inv x = 0) ==> ((x < 1) \/ (inv x = 1))`
+	by (RW_TAC posreal_ss []
+	    ++ `1 - inv x <= 0` by RW_TAC posreal_ss [le_zero]
+	    ++ `~(1=infty)` by RW_TAC posreal_ss []
+	    ++ `1 <= 0 + inv x` by METIS_TAC [sub_le_eq]
+	    ++  FULL_SIMP_TAC std_ss [add_lzero, inv_one_le]
+	    ++ METIS_TAC [preal_lt_def, le_total, le_antisym])
+   ++ FULL_SIMP_TAC posreal_ss []
+   ++ METIS_TAC []);
+
+val bound1_eq_lemma = store_thm
+  ("bound1_eq_lemma",
+   ``!x y. (~(y=infty)) ==> ((bound1 x) * y + (1 - bound1 x) * y = y)``,
+   RW_TAC posreal_ss [bound1_def, sub_rdistrib, sub_add2]
+   ++ `1 < infty` by RW_TAC posreal_ss [preal_lt_def]
+   ++ `~(x = infty)` by METIS_TAC [let_trans, infty_le, preal_lt_def]
+   ++ `~(x*y = infty)` by METIS_TAC [mul_eq_infty]
+   ++ METIS_TAC [sub_add2, le_refl, operand_le_one_imp_mul_le_one]);
+
+(* -------------------------- general wp proofs ---------------------------- *)
+
 val seq_term = store_thm
   ("seq_term",
   ``!a b. ((wp a One) = One) /\ ((wp b One) = One) ==> ((wp (Seq a b) One) = One)``,
   RW_TAC std_ss [wp_def]);
 
-val demon_term = store_thm
-  ("demon_term",
-   ``!a b. ((wp a One) = One) /\ ((wp b One) = One) ==> ((wp (Demon a b) One) = One)``,
+val Nondet_term = store_thm
+  ("Nondet_term",
+   ``!a b. ((wp a One) = One) /\ ((wp b One) = One) ==> ((wp (Nondet a b) One) = One)``,
    RW_TAC posreal_ss [wp_def, Min_def, One_def]);
-
-val Demonchoice_term = store_thm
-  ("Demonchoice_term",
-   ``!v l. ((LENGTH l) > 0) ==> ((wp (Demonchoice v l) One) = One)``,
-   RW_TAC std_ss [Demonchoice_def]
-   ++ Induct_on `l`
-   ++ RW_TAC arith_ss [LENGTH]
-   ++ Cases_on `l`
-   >> RW_TAC posreal_ss [MAP, Demons_def, wp_def, One_def, Min_def, min_def]
-   ++ FULL_SIMP_TAC arith_ss [LENGTH]
-   ++ Cases_on `t`
-   ++ FULL_SIMP_TAC arith_ss [LENGTH, MAP, Demons_def]
-   ++ MATCH_MP_TAC demon_term
-   ++ RW_TAC posreal_ss [wp_def, One_def]);
-
-val set_payer_term = store_thm
-  ("set_payer_term",
-   ``!n. (n > 0) ==> ((wp (set_payer n) One) = One)``,
-   RW_TAC std_ss [set_payer_def]
-   ++ MATCH_MP_TAC Demonchoice_term
-   ++ RW_TAC arith_ss [zero_to_n_Int_list_length]);
 
 val wp_1bounded_exp_is_1bounded = store_thm
   ("wp_1bounded_exp_is_1bounded",
@@ -299,13 +354,6 @@ val wp_1bounded_exp_is_1bounded = store_thm
 ++ MATCH_MP_TAC healthy_bounded
 ++ RW_TAC posreal_ss [wp_healthy]);
 
-val min_leq = store_thm
-  ("min_leq",
-   ``!e f g. Leq f e /\ Leq g e ==> Leq (Min f g) e``,
-   RW_TAC real_ss [Leq_def, Min_def, preal_min_def]
-   ++ Cases_on `f s <= g s`
-   ++ RW_TAC posreal_ss []);
-
 val strip_nested_min = store_thm
   ("strip_nested_min",
    ``!x y. min x (min x y) = min x y``,
@@ -314,20 +362,90 @@ val strip_nested_min = store_thm
    ++ RW_TAC posreal_ss [preal_min_def]
    ++ FULL_SIMP_TAC posreal_ss []);
 
-val Demonchoice_result = store_thm
-  ("Demonchoice_result",
+val NondetAssign_term = store_thm
+  ("NondetAssign_term",
+   ``!v l. ((LENGTH l) > 0) ==> ((wp (NondetAssign v l) One) = One)``,
+   RW_TAC std_ss [NondetAssign_def]
+   ++ Induct_on `l`
+   ++ RW_TAC arith_ss [LENGTH]
+   ++ Cases_on `l`
+   >> RW_TAC posreal_ss [MAP, Nondets_def, wp_def, One_def, Min_def, min_def]
+   ++ FULL_SIMP_TAC arith_ss [LENGTH]
+   ++ Cases_on `t`
+   ++ FULL_SIMP_TAC arith_ss [LENGTH, MAP, Nondets_def]
+   ++ MATCH_MP_TAC Nondet_term
+   ++ RW_TAC posreal_ss [wp_def, One_def]);
+
+val NondetAssign_repeat_list = store_thm
+  ("NondetAssign_repeat_list",
+``!v (l:'a list) (x:'a). (!x'. (MEM x' l) ==> (x' = x)) /\
+	 (LENGTH l > 0) ==>
+	 (wp (NondetAssign v l) = wp (NondetAssign v [x]))``,
+   REPEAT STRIP_TAC
+   ++ Induct_on `l`
+   ++ RW_TAC std_ss [LENGTH]
+   ++ Cases_on `l`
+   >> (`h=x` by METIS_TAC [MEM]
+       ++ ASM_REWRITE_TAC [])
+   ++ FULL_SIMP_TAC std_ss [LENGTH]
+   ++ `!x'. (MEM x' (h'::t)) ==> (x' = x)`
+	by METIS_TAC [MEM]
+   ++ FULL_SIMP_TAC std_ss [NondetAssign_def, MAP, Nondets_def]
+   ++ SIMP_TAC std_ss [wp_def]
+   ++ `h = x` by METIS_TAC [MEM]
+   ++ ASM_REWRITE_TAC []
+   ++ SIMP_TAC std_ss [wp_def, FUN_EQ_THM, refl_min]);
+
+val NondetAssign_of_singleton_Leq = store_thm
+  ("NondetAssign_of_singleton_Leq",
+   ``!v k (l:'a list) (x:'a). (MEM x l) ==>
+	Leq (wp (NondetAssign v l) (\s. if ~(s v = k) then 1 else 0))
+	    (wp (NondetAssign v [x])(\s. if ~(s v = k) then 1 else 0))``,
+   REPEAT STRIP_TAC
+   ++ Induct_on `l`
+   >> RW_TAC std_ss [MEM]
+   ++ RW_TAC std_ss [MEM]
+   >> (Cases_on `l`
+       >> SIMP_TAC std_ss [leq_refl]
+       ++ FULL_SIMP_TAC std_ss [NondetAssign_def, MAP, Nondets_def, wp_def, Leq_def]
+       ++ RW_TAC posreal_ss [Min_def, preal_min_def]
+       ++ `expect1 (\(s:string->'a). (if ~(s v = k) then (1:posreal) else 0))` 
+   	by (RW_TAC posreal_ss [expect1_def]
+   	    ++ RW_TAC posreal_ss [zero_le, le_refl])
+       ++ `expect1 (wp (Nondets (Assign v (\s. h')::MAP (\x. Assign v (\s. x)) t))
+      		       (\s. (if ~(s v = k) then 1 else 0)))`
+	by METIS_TAC [expect1_postE_imp_expect1_wp_postE]
+       ++ FULL_SIMP_TAC std_ss [expect1_def])
+   ++ Cases_on `l`
+   >> FULL_SIMP_TAC std_ss [MEM]
+   ++ FULL_SIMP_TAC std_ss [NondetAssign_def, MAP, Nondets_def, wp_def, Leq_def]
+   ++ RW_TAC posreal_ss [Min_def, preal_min_def]
+   << [FULL_SIMP_TAC std_ss [assign_eta]
+       ++ `~((1:posreal) <= 0)` by RW_TAC posreal_ss []
+       ++ METIS_TAC [le_trans],
+       `expect1 (\(s:string->'a). (if ~(s v = k) then (1:posreal) else 0))` 
+		by (RW_TAC posreal_ss [expect1_def]
+		    ++ RW_TAC posreal_ss [zero_le, le_refl])
+       ++ `expect1 (wp (Nondets (Assign v (\s. h')::MAP (\x. Assign v (\s. x)) t))
+      		       (\s. (if ~(s v = k) then 1 else 0)))`
+		by METIS_TAC [expect1_postE_imp_expect1_wp_postE]
+       ++ FULL_SIMP_TAC std_ss [expect1_def],
+       FULL_SIMP_TAC std_ss [assign_eta, le_zero]]);
+
+val NondetAssign_partial_result = store_thm
+  ("NondetAssign_partial_result",
    ``!v l k. ((LENGTH l) > 0) ==>
-	((wp (Demonchoice v l) (\s. if (MEM (s v) l) then 1 else 0)) = One) /\
+	((wp (NondetAssign v l) (\s. if (MEM (s v) l) then 1 else 0)) = One) /\
 	((?x y. (MEM x l) /\ (MEM y l) /\ (~(x=y))) ==>
-	 	((wp (Demonchoice v l) (\s. if ((s v) = k) then 1 else 0)) = Zero))``,
-   RW_TAC std_ss [Demonchoice_def]
+	 	((wp (NondetAssign v l) (\s. if ((s v) = k) then 1 else 0)) = Zero))``,
+   RW_TAC std_ss [NondetAssign_def]
    << [Induct_on `l`
    	++ RW_TAC arith_ss [LENGTH]
     	++ Cases_on `l`
-    	>> RW_TAC posreal_ss [MAP, Demons_def, wp_def, assign_eta, One_def, MEM]
-    	++ FULL_SIMP_TAC arith_ss [LENGTH, MAP, Demons_def, MEM]
+    	>> RW_TAC posreal_ss [MAP, Nondets_def, wp_def, assign_eta, One_def, MEM]
+    	++ FULL_SIMP_TAC arith_ss [LENGTH, MAP, Nondets_def, MEM]
     	++ RW_TAC posreal_ss [wp_def, assign_eta]
-    	++ Q.ABBREV_TAC `prog = (Demons (Assign v (\s. h')::MAP (\x. Assign v (\s. x)) t))`
+    	++ Q.ABBREV_TAC `prog = (Nondets (Assign v (\s. h')::MAP (\x. Assign v (\s. x)) t))`
    	++ `Leq (wp prog (\s. (if (s v = h') \/ MEM (s v) t then 1 else 0)))
      		(wp prog (\s. (if (s v = h) \/ (s v = h') \/ MEM (s v) t then 1 else 0)))` by
 		(MATCH_MP_TAC wp_mono
@@ -351,124 +469,1236 @@ val Demonchoice_result = store_thm
 	++ FULL_SIMP_TAC arith_ss [LENGTH, MEM]
 	++ Cases_on `t`
 	++ FULL_SIMP_TAC arith_ss [LENGTH, MEM]
-	++ FULL_SIMP_TAC posreal_ss [MAP, Demons_def, wp_def, assign_eta, Min_def, Zero_def]
+	++ FULL_SIMP_TAC posreal_ss [MAP, Nondets_def, wp_def, assign_eta, Min_def, Zero_def]
 	++ REPEAT STRIP_TAC 
 	++ RW_TAC posreal_ss [strip_nested_min]
 	++ FULL_SIMP_TAC posreal_ss []]);
 
-val Demonchoice_do_nothing = store_thm
-  ("Demonchoice_do_nothing",
+val NondetAssign_result = store_thm
+  ("NondetAssign_result",
+   ``!v l k. ((LENGTH l) > 0) ==>
+	((wp (NondetAssign v l) (\s. if (MEM (s v) l) then 1 else 0)) = One) /\
+	((?x y. (MEM x l) /\ (MEM y l) /\ (~(x=y))) ==>
+	 	((wp (NondetAssign v l) (\s. if ((s v) = k) then 1 else 0)) = Zero) /\
+                ((MEM k l) ==> ((wp (NondetAssign v l) (\s. if ~((s v) = k) then 1 else 0)) = Zero)))``,
+   RW_TAC std_ss []
+   << [RW_TAC std_ss [NondetAssign_def]
+	++ Induct_on `l`
+   	++ RW_TAC arith_ss [LENGTH]
+    	++ Cases_on `l`
+    	>> RW_TAC posreal_ss [MAP, Nondets_def, wp_def, assign_eta, One_def, MEM]
+    	++ FULL_SIMP_TAC arith_ss [LENGTH, MAP, Nondets_def, MEM]
+    	++ RW_TAC posreal_ss [wp_def, assign_eta]
+    	++ Q.ABBREV_TAC `prog = (Nondets (Assign v (\s. h')::MAP (\x. Assign v (\s. x)) t))`
+   	++ `Leq (wp prog (\s. (if (s v = h') \/ MEM (s v) t then 1 else 0)))
+     		(wp prog (\s. (if (s v = h) \/ (s v = h') \/ MEM (s v) t then 1 else 0)))` by
+		(MATCH_MP_TAC wp_mono
+		++ RW_TAC posreal_ss [Leq_def]
+		++ Cases_on `(s v = h') \/ MEM (s v) t`
+		++ RW_TAC bool_ss []
+		++ RW_TAC posreal_ss [leq_refl])
+   	++ `Leq (wp prog (\s. (if (s v = h) \/ (s v = h') \/ MEM (s v) t then 1 else 0))) One` by
+		(MATCH_MP_TAC wp_1bounded_exp_is_1bounded
+		++ RW_TAC posreal_ss [Leq_def, One_def]
+		++ Cases_on `(s v = h) \/ (s v = h') \/ MEM (s v) t`
+		++ RW_TAC bool_ss []
+		++ RW_TAC posreal_ss [leq_refl])
+   	++ `Leq One (wp prog (\s. (if (s v = h) \/ (s v = h') \/ MEM (s v) t then 1 else 0)))` by
+		METIS_TAC [leq_refl, leq_trans]
+   	++ `(wp prog (\s. (if (s v = h) \/ (s v = h') \/ MEM (s v) t then 1 else 0))) = One` by 		
+	 	METIS_TAC [leq_antisym]
+   	++ RW_TAC posreal_ss [Min_def, One_def],
+	RW_TAC std_ss [NondetAssign_def]
+	++ Induct_on `l`
+	++ FULL_SIMP_TAC arith_ss [LENGTH, MEM]
+	++ Cases_on `l`
+	++ FULL_SIMP_TAC arith_ss [LENGTH, MEM]
+	++ Cases_on `t`
+	++ FULL_SIMP_TAC arith_ss [LENGTH, MEM]
+	++ FULL_SIMP_TAC posreal_ss [MAP, Nondets_def, wp_def, assign_eta, Min_def, Zero_def]
+	++ REPEAT STRIP_TAC 
+	++ RW_TAC posreal_ss [strip_nested_min]
+	++ FULL_SIMP_TAC posreal_ss [],
+	Suff `Leq (wp (NondetAssign v l) (\s. (if ~(s v = k) then 1 else 0)))
+		   Zero`
+	>> METIS_TAC [leq_zero]
+	++ `Leq (wp (NondetAssign v l) (\s. if ~(s v = k) then 1 else 0))
+	    	(wp (NondetAssign v [k])(\s. if ~(s v = k) then 1 else 0))`
+		by METIS_TAC [NondetAssign_of_singleton_Leq]
+	++ FULL_SIMP_TAC std_ss [NondetAssign_def, MAP, wp_def, assign_eta, Nondets_def, Zero_def]
+	++ RW_TAC posreal_ss []]);
+
+val NondetAssign_do_nothing = store_thm
+  ("NondetAssign_do_nothing",
    ``!v l e. (LENGTH l > 0) ==>
 	        ((!a s. e s = e (assign v a s)) ==>
-		   ((wp (Demonchoice v l) e) = e))``,
+		   ((wp (NondetAssign v l) e) = e))``,
    REPEAT STRIP_TAC
-   ++ RW_TAC std_ss [Demonchoice_def]
+   ++ RW_TAC std_ss [NondetAssign_def]
    ++ Induct_on `l`
    >> RW_TAC std_ss [LENGTH]
    ++ Cases_on `l`
-   << [RW_TAC std_ss [LENGTH, MAP, Demons_def, wp_def]
+   << [RW_TAC std_ss [LENGTH, MAP, Nondets_def, wp_def]
        ++ METIS_TAC [],
-       FULL_SIMP_TAC posreal_ss [LENGTH, MAP, Demons_def, wp_def, Min_def]
+       FULL_SIMP_TAC posreal_ss [LENGTH, MAP, Nondets_def, wp_def, Min_def]
        ++ METIS_TAC [min_refl]]);
 
-val LESS_EQ_EQ_LESS_SUC = store_thm
-  ("LESS_EQ_EQ_LESS_SUC",
-   ``!n m. (n <= m) = (n < SUC m)``,
-   RW_TAC arith_ss []);
+val NondetAssign_do_nothing_val = store_thm
+  ("NondetAssign_do_nothing_val",
+   ``!v (l:value list) (e:(string->value)->posreal). (LENGTH l > 0) ==>
+	        ((!a s. e s = e (assign v a s)) ==>
+		   ((wp (NondetAssign v l) e) = e))``,
+   REPEAT STRIP_TAC
+   ++ RW_TAC std_ss [NondetAssign_def]
+   ++ Induct_on `l`
+   >> RW_TAC std_ss [LENGTH]
+   ++ Cases_on `l`
+   << [RW_TAC std_ss [LENGTH, MAP, Nondets_def, wp_def]
+       ++ METIS_TAC [],
+       FULL_SIMP_TAC posreal_ss [LENGTH, MAP, Nondets_def, wp_def, Min_def]
+       ++ METIS_TAC [min_refl]]);
 
-val set_payer_result = store_thm
-  ("set_payer_result",
-   ``!n k. 
-	(n>0) ==>
-		(((wp (set_payer n) (\s.if ((num_of_value(s"payer")) <= n) then 1 else 0)) = One) /\
-  		 ((wp (set_payer n) (\s.if (s"payer"=k) then 1 else 0)) = Zero))``,
-   STRIP_TAC
-   ++ STRIP_TAC
-   ++ `((LENGTH (zero_to_n_Int_list (SUC n))) > 0) ==>
-	((wp (Demonchoice "payer" (zero_to_n_Int_list (SUC n))) 
-             (\s. if (MEM (s "payer") (zero_to_n_Int_list (SUC n))) then 1 else 0)) = One) /\
-	((?x y. (MEM x (zero_to_n_Int_list (SUC n))) /\ 
-                (MEM y (zero_to_n_Int_list (SUC n))) /\ 
-                (~(x=y))) ==>
-	 	((wp (Demonchoice "payer" (zero_to_n_Int_list (SUC n))) 
-                     (\s. if ((s "payer") = k) then 1 else 0)) = Zero))` 
-      by METIS_TAC [Demonchoice_result]
-   ++ FULL_SIMP_TAC std_ss [zero_to_n_Int_list_length]
-   ++ RW_TAC std_ss [set_payer_def]
-   << [`(wp (Demonchoice "payer" (zero_to_n_Int_list (SUC n)))
-            (\s. (if num_of_value (s "payer") <= n then 1 else 0))) =
-        (wp (Demonchoice "payer" (zero_to_n_Int_list (SUC n)))
-            (\s. (if num_of_value (s "payer") < SUC n then 1 else 0)))` 
-       by RW_TAC arith_ss [LESS_EQ_EQ_LESS_SUC]
-       ++ `Leq (\s. (if MEM (s "payer") (zero_to_n_Int_list (SUC n)) then 1 else 0))
-               (\s. (if num_of_value (s "payer") < SUC n then 1 else 0))`
-       by (RW_TAC posreal_ss [Leq_def]
-           ++ Cases_on `MEM (s "payer") (zero_to_n_Int_list (SUC n))`
-           ++ RW_TAC posreal_ss [zero_to_n_Int_list_contains_Int])
-       ++ `Leq  (wp (Demonchoice "payer" (zero_to_n_Int_list (SUC n)))
-                    (\s. (if MEM (s "payer") (zero_to_n_Int_list (SUC n)) then 1 else 0)))
-                (wp (Demonchoice "payer" (zero_to_n_Int_list (SUC n)))
-                    (\s. (if num_of_value (s "payer") < SUC n then 1 else 0)))` 
-          by METIS_TAC [wp_mono]
-       ++ `Leq One 
-               (wp (Demonchoice "payer" (zero_to_n_Int_list (SUC n)))
-                   (\s. (if num_of_value (s "payer") <= n then 1 else 0)))` 
-          by METIS_TAC []
-       ++ `Leq (\s. (if num_of_value (s "payer") <= n then 1 else 0)) One`
-          by (RW_TAC posreal_ss [Leq_def, One_def]
-              ++ Cases_on `num_of_value (s "payer") <= n`
-              ++ RW_TAC posreal_ss [])
-       ++ `Leq (wp (Demonchoice "payer" (zero_to_n_Int_list (SUC n)))
-                   (\s. (if num_of_value (s "payer") <= n then 1 else 0)))
-               One` 
-          by METIS_TAC [wp_1bounded_exp_is_1bounded]
-       ++ METIS_TAC [leq_antisym],
-       `(?x y. MEM x (zero_to_n_Int_list (SUC n)) /\
-               MEM y (zero_to_n_Int_list (SUC n)) /\ 
-               ~(x = y))`
-       by (`MEM (Int (&0)) (zero_to_n_Int_list (SUC n))` 
-           by RW_TAC arith_ss [zero_to_n_Int_list_contains]
-           ++ `MEM (Int (&1)) (zero_to_n_Int_list (SUC n))` 
-           by RW_TAC arith_ss [zero_to_n_Int_list_contains]
-           ++  `~((Int 0) = (Int 1))` 
-           by RW_TAC int_ss []
-           ++ METIS_TAC [])
-       ++ METIS_TAC []]);
+val ProbAssign_do_nothing = store_thm
+  ("ProbAssign_do_nothing",
+   ``!v l e. (LENGTH l > 0) ==>
+	        ((!a s. e s = e (assign v a s)) ==>
+		   ((wp (ProbAssign v l) e) = e))``,
+   REPEAT STRIP_TAC
+   ++ RW_TAC std_ss []
+   ++ Induct_on `l`
+   >> RW_TAC std_ss [LENGTH]
+   ++ FULL_SIMP_TAC posreal_ss [LENGTH, MAP, ProbAssign_def, Probs_def, wp_def, lin_eta, FUN_EQ_THM, preal_div_def]
+       ++ Cases_on `LENGTH l > 0`
+       >> (FULL_SIMP_TAC std_ss [LENGTH]
+	   ++ RW_TAC list_ss [MAP_MAP_o]
+	   ++ RW_TAC posreal_ss [preal_div_def]
+	   ++ `inv (& (SUC (LENGTH l))) *
+               inv (1 - inv (& (SUC (LENGTH l)))) =
+	       inv ((& (SUC (LENGTH l))) * (1 - inv (& (SUC (LENGTH l)))))`
+		by (`~((& (SUC (LENGTH l)) * (1 - inv (& (SUC (LENGTH l))))) = (0:posreal))`
+			by RW_TAC posreal_ss [entire, posreal_of_num_inj, 
+					      subr1_inv_eq_zero, DE_MORGAN_THM]
+		    ++ METIS_TAC [inv_mul])
+	   ++ RW_TAC std_ss []
+	   ++ POP_ASSUM (K ALL_TAC)
+	   ++ `~ (& (SUC (LENGTH l)) = (0:posreal))`
+		by RW_TAC arith_ss [posreal_of_num_inj]
+	   ++ RW_TAC posreal_ss [sub_ldistrib, mul_rinv]
+	   ++ `e (assign v (\s. h) x) = e x` by METIS_TAC []
+	   ++ RW_TAC std_ss []
+	   ++ Q.UNABBREV_TAC `x'`
+	   ++ Cases_on `e x = infty`
+	   >> (`~(bound1 (inv (& (SUC (LENGTH l)))) = 0)` by RW_TAC posreal_ss [bound1_def]
+	       ++ RW_TAC posreal_ss [mul_rinfty, add_rinfty])
+	   ++ METIS_TAC [bound1_eq_lemma])
+	++ Cases_on `l`
+	>> (RW_TAC posreal_ss [MAP, Probs_def, wp_def, Zero_def, mul_rzero, add_rzero]
+	    ++ Q.UNABBREV_TAC `x'`
+	    ++ RW_TAC posreal_ss [LENGTH])
+	++ FULL_SIMP_TAC arith_ss [LENGTH]);
+
+val ProbAssign_do_nothing_val = store_thm
+  ("ProbAssign_do_nothing_val",
+   ``!v l e. (LENGTH l > 0) ==>
+	        ((!a (s:string->value). e s = e (assign v a s)) ==>
+		   ((wp (ProbAssign v l) e) = e))``,
+   REPEAT STRIP_TAC
+   ++ RW_TAC std_ss []
+   ++ Induct_on `l`
+   >> RW_TAC std_ss [LENGTH]
+   ++ FULL_SIMP_TAC posreal_ss [LENGTH, MAP, ProbAssign_def, Probs_def, wp_def, lin_eta, FUN_EQ_THM, preal_div_def]
+       ++ Cases_on `LENGTH l > 0`
+       >> (FULL_SIMP_TAC std_ss [LENGTH]
+	   ++ RW_TAC list_ss [MAP_MAP_o]
+	   ++ RW_TAC posreal_ss [preal_div_def]
+	   ++ `inv (& (SUC (LENGTH l))) *
+               inv (1 - inv (& (SUC (LENGTH l)))) =
+	       inv ((& (SUC (LENGTH l))) * (1 - inv (& (SUC (LENGTH l)))))`
+		by (`~((& (SUC (LENGTH l)) * (1 - inv (& (SUC (LENGTH l))))) = (0:posreal))`
+			by RW_TAC posreal_ss [entire, posreal_of_num_inj, 
+					      subr1_inv_eq_zero, DE_MORGAN_THM]
+		    ++ METIS_TAC [inv_mul])
+	   ++ RW_TAC std_ss []
+	   ++ POP_ASSUM (K ALL_TAC)
+	   ++ `~ (& (SUC (LENGTH l)) = (0:posreal))`
+		by RW_TAC arith_ss [posreal_of_num_inj]
+	   ++ RW_TAC posreal_ss [sub_ldistrib, mul_rinv]
+	   ++ `e (assign v (\s. h) x) = e x` by METIS_TAC []
+	   ++ RW_TAC std_ss []
+	   ++ Q.UNABBREV_TAC `x'`
+	   ++ Cases_on `e x = infty`
+	   >> (`~(bound1 (inv (& (SUC (LENGTH l)))) = 0)` by RW_TAC posreal_ss [bound1_def]
+	       ++ RW_TAC posreal_ss [mul_rinfty, add_rinfty])
+	   ++ METIS_TAC [bound1_eq_lemma])
+	++ Cases_on `l`
+	>> (RW_TAC posreal_ss [MAP, Probs_def, wp_def, Zero_def, mul_rzero, add_rzero]
+	    ++ Q.UNABBREV_TAC `x'`
+	    ++ RW_TAC posreal_ss [LENGTH])
+	++ FULL_SIMP_TAC arith_ss [LENGTH]);
+	   
+(* -------------------------- set_payer proofs ----------------------------- *)
+
+val set_payer_term = store_thm
+  ("set_payer_term",
+   ``!n nsapays. (n > 0) ==> ((wp (set_payer n nsapays) One) = One)``,
+   RW_TAC std_ss [set_payer_def]
+   >> RW_TAC posreal_ss [wp_def, One_def]
+   ++ MATCH_MP_TAC NondetAssign_term
+   ++ RW_TAC arith_ss [zero_to_n_Int_list_length]);
+
+(* -------------------------- initialize proofs ---------------------------- *)
 
 val initialize_term = store_thm
   ("initialize_term",
-   ``!n. (n > 0) ==> ((wp (initialize n) One) = One)``,
+   ``!n. (n > 0) ==> ((wp (initialize n nsapays) One) = One)``,
    RW_TAC std_ss [initialize_def, Program_def]
-   ++ METIS_TAC [seq_term, initialize_var_N_term, set_payer_term]);
+   ++ METIS_TAC [seq_term, initialize_var_N_term, initialize_var_NSApays_term, set_payer_term]);
 
-(*
 val initialize_result = store_thm
   ("initialize_result",
-   ``!n k. (n > 0) ==> 
-	((wp (initialize n) 
-	     (\s.if ((num_of_value(s"N")) = n) then 1 else 0)) = One) /\
-	((wp (initialize n) 
-             (\s.if ((0<=(num_of_value(s"payer")))/\((num_of_value(s"payer"))<=n)) then 1 else 0)) = One) /\
-	((wp (initialize n) 
- 	     (\s.if ((num_of_value(s"payer"))=k) then 1 else 0)) = Zero)``,
-   ????);
+   ``!n nsapays k. (n > 0) ==>
+	((wp (initialize n nsapays) (\s. if ((num_of_value (s "N")) = n) then 1 else 0) = One) /\
+	 (wp (initialize n nsapays) (\s. if nsapays 
+					 then (if ((s "NSApays") = Yes) then 1 else 0)								 else (if ((s "NSApays") = No) then 1 else 0)) = One) /\
+	 (if nsapays
+	  then (wp (initialize n nsapays) (\s. if ((s "payer") = (s "N")) then 1 else 0) = One)
+	  else 
+	  ((wp (initialize n nsapays) 
+	       (\s. if ((num_of_value (s "payer")) < 
+		        (num_of_value (s "N"))) then 1 else 0) = One)
+	    /\ ((n > 1) ==> ((wp (initialize n nsapays)
+			         (\s. if (s "payer") = Int (& k) then 1 else 0) = Zero)
+	    		     /\ ( (k < n) ==>
+				(wp (initialize n nsapays)
+				    (\s. if ~ ((s "payer") = Int (& k)) 
+					 then 1 else 0) = Zero)))))))``,
+   REPEAT STRIP_TAC
+   << [RW_TAC std_ss [initialize_def, Program_def, wp_def, set_payer_def, 
+		   initialize_var_NSApays_def, assign_eta]
+    >> RW_TAC posreal_ss [initialize_var_N_result]
+    ++ `wp (NondetAssign "payer" (zero_to_n_Int_list n))
+	   (\s. (if num_of_value (s "N") = n then 1 else 0)) =
+	   (\s. (if num_of_value (s "N") = n then 1 else 0))`
+	by (`LENGTH (zero_to_n_Int_list n) > 0`
+		by (Cases_on `n`
+	    	    ++ RW_TAC arith_ss [zero_to_n_Int_list, LENGTH_SNOC])
+	    ++ `!(n:num). (n > 0) ==>
+		(?(l:value list). l = zero_to_n_Int_list n)`
+		by (Induct_on `n`
+	    	    ++ RW_TAC arith_ss [])
+	    ++ `?l. zero_to_n_Int_list n = l` by METIS_TAC []
+	    ++ `LENGTH l > 0` by RW_TAC arith_ss []
+	    ++ ASM_REWRITE_TAC []
+	    ++ `!a s. (\s. (if num_of_value (s "N") = n then (1:posreal) else 0)) s =
+		      (\s. (if num_of_value (s "N") = n then 1 else 0))
+		      (assign "payer" a s)` 
+		by RW_TAC std_ss [assign_eta]
+	    ++ `!(v :string) (l :value list) (e :(string -> value) -> posreal).
+         	 LENGTH l > (0 :num) ==>
+         	 (!(a :(string -> value) -> value) (s :string -> value).
+          	 e s = e (assign v a s)) ==>
+         	(wp (NondetAssign v l) e = e)` 
+		by METIS_TAC [NondetAssign_do_nothing_val]
+	    ++ FULL_SIMP_TAC std_ss [])
+    ++ RW_TAC std_ss [initialize_var_N_result],
+    RW_TAC std_ss [initialize_def, Program_def, wp_def, set_payer_def, assign_eta]
+    >> (`wp (initialize_var_NSApays T)
+              		(\s. (if T then
+                    		(if s "NSApays" = Yes then 1 else 0)
+                  	      else
+                    		(if s "NSApays" = No then 1 else 0))) = One`
+			by METIS_TAC [Q.SPECL [`T`] initialize_var_NSApays_result]
+	++ FULL_SIMP_TAC std_ss [initialize_var_N_term])
+    ++ `wp (NondetAssign "payer" (zero_to_n_Int_list n))
+	   (\s. (if s "NSApays" = No then 1 else 0)) =
+	   (\s. (if s "NSApays" = No then 1 else 0))`
+	by (`LENGTH (zero_to_n_Int_list n) > 0`
+		by (Cases_on `n`
+	    	    ++ RW_TAC arith_ss [zero_to_n_Int_list, LENGTH_SNOC])
+	    ++ `!(n:num). (n > 0) ==>
+		(?(l:value list). l = zero_to_n_Int_list n)`
+		by (Induct_on `n`
+	    	    ++ RW_TAC arith_ss [])
+	    ++ `?l. zero_to_n_Int_list n = l` by METIS_TAC []
+	    ++ `LENGTH l > 0` by RW_TAC arith_ss []
+	    ++ ASM_REWRITE_TAC []
+	    ++ `!a s. (\s. (if s "NSApays" = No then (1:posreal) else 0)) s =
+		      (\s. (if s "NSApays" = No then 1 else 0))
+		      (assign "payer" a s)` 
+		by RW_TAC std_ss [assign_eta]
+	    ++ `!(v :string) (l :value list) (e :(string -> value) -> posreal).
+         	 LENGTH l > (0 :num) ==>
+         	 (!(a :(string -> value) -> value) (s :string -> value).
+          	 e s = e (assign v a s)) ==>
+         	(wp (NondetAssign v l) e = e)` 
+		by METIS_TAC [NondetAssign_do_nothing_val]
+	    ++ FULL_SIMP_TAC std_ss [])
+    ++ ASM_REWRITE_TAC []
+    ++ POP_ASSUM (K ALL_TAC)
+    ++ `wp (initialize_var_NSApays F)
+           (\s. (if F then
+                    (if s "NSApays" = Yes then 1 else 0)
+                 else
+                    (if s "NSApays" = No then 1 else 0))) = One`
+	by METIS_TAC [Q.SPECL [`F`] initialize_var_NSApays_result]
+    ++ FULL_SIMP_TAC std_ss [initialize_var_N_term],
+    RW_TAC std_ss []
+    << [RW_TAC posreal_ss [initialize_def, Program_def, wp_def, set_payer_def, assign_eta,
+			   initialize_var_NSApays_def, initialize_var_N_def, One_def],
+ 	RW_TAC posreal_ss [initialize_def, Program_def, wp_def, set_payer_def, assign_eta, 
+			   initialize_var_NSApays_def, initialize_var_N_def]
+	++ `Leq (\s. (if n = num_of_value (s "N") then 1 else 0))
+		(wp (NondetAssign "payer" (zero_to_n_Int_list n))
+	    	    (\s. (if num_of_value (s "payer") < num_of_value (s "N") then 1 else 0)))`
+		by (`Leq (wp (NondetAssign "payer" (zero_to_n_Int_list n))
+	    		     (\s. (if n = num_of_value (s "N") then 1 else 0)))
+			 (wp (NondetAssign "payer" (zero_to_n_Int_list n))
+	    		     (\s. (if num_of_value (s "payer") < num_of_value (s "N") then 1 else 0)))`
+			by (`Leq (Conj (wp (NondetAssign "payer" (zero_to_n_Int_list n)) 
+		  			   (\s. if (n = num_of_value (s "N")) then 1 else 0))
+	      			       (wp (NondetAssign "payer" (zero_to_n_Int_list n))
+		  			   (\s. if MEM (s "payer") (zero_to_n_Int_list n) then 1 else 0)))
+				 (wp (NondetAssign "payer" (zero_to_n_Int_list n))
+	    			     (\s. if num_of_value (s "payer") < num_of_value (s "N") then 1 else 0))`
+				by (`Leq (Conj (wp (NondetAssign "payer" (zero_to_n_Int_list n))
+			   			   (\s. (if n = num_of_value (s "N") then 1 else 0)))
+		       			       (wp (NondetAssign "payer" (zero_to_n_Int_list n))
+			   			   (\s. (if MEM (s "payer") (zero_to_n_Int_list n) 
+						         then 1 else 0))))
+		 			 (wp (NondetAssign "payer" (zero_to_n_Int_list n))
+		     			     (Conj (\s. if (n = num_of_value (s "N")) then 1 else 0)
+	      		   			   (\s. if MEM (s "payer") (zero_to_n_Int_list n) 
+							then (1:posreal) else 0)))`
+					by METIS_TAC [wp_conj]
+	    			    ++ Suff `Leq (wp (NondetAssign "payer" (zero_to_n_Int_list n))
+		     	     			     (Conj (\s. if (n = num_of_value (s "N")) then 1 else 0)
+	      		   	   			   (\s. if MEM (s "payer") (zero_to_n_Int_list n) 
+								then (1:posreal) else 0)))
+	    		 			 (wp (NondetAssign "payer" (zero_to_n_Int_list n))
+	    		     			     (\s. if num_of_value (s "payer") < num_of_value (s "N") 
+							  then 1 else 0))`
+	    			    >> PROVE_TAC [leq_trans]
+	    			    ++ POP_ASSUM (K ALL_TAC)
+	    			    ++ MATCH_MP_TAC wp_mono
+	    			    ++ `Leq (\s. if MEM (s "payer") 
+						        (zero_to_n_Int_list (num_of_value (s "N"))) 
+						 then 1 else 0)
+        	    			    (\s. if num_of_value (s "payer") < num_of_value (s "N") 
+						 then (1:posreal) else 0)`
+					by (RW_TAC posreal_ss [Leq_def]
+	    				    ++ RW_TAC posreal_ss [zero_le, le_refl]
+	  			  	    ++ METIS_TAC [zero_to_n_Int_list_contains_Int])
+	    			    ++ `Leq (\s. if MEM (s "payer") (zero_to_n_Int_list n) /\ 
+			 			    (n = num_of_value (s "N")) then 1 else 0)
+		    			    (\s. if MEM (s "payer") 
+						    (zero_to_n_Int_list (num_of_value (s "N"))) 
+						 then 1 else 0)`
+					by (RW_TAC posreal_ss [Leq_def]
+	     			            ++ RW_TAC posreal_ss [zero_le, le_refl]
+	       			            ++ METIS_TAC [])
+				    ++ `Leq (Conj (\s. if (n = num_of_value (s "N")) then 1 else 0)
+	 			     		  (\s. if MEM (s "payer") (zero_to_n_Int_list n) 
+						       then (1:posreal) else 0))
+					    (\s. if MEM (s "payer") (zero_to_n_Int_list n) /\ 
+						    (n = num_of_value (s "N")) then 1 else 0)`
+					by (RW_TAC posreal_ss [Leq_def, Conj_def]
+					    ++ RW_TAC posreal_ss []
+					    ++ METIS_TAC [])
+				    ++ PROVE_TAC [leq_trans])
+			    ++ `LENGTH (zero_to_n_Int_list n) > 0`
+				by (Cases_on `n`
+				    ++ RW_TAC arith_ss [zero_to_n_Int_list, LENGTH_SNOC])
+		  	    ++ `wp (NondetAssign "payer" (zero_to_n_Int_list n))
+	       			   (\s. (if MEM (s "payer") (zero_to_n_Int_list n) then 1 else 0)) = One`
+				by METIS_TAC [NondetAssign_partial_result]
+			    ++ FULL_SIMP_TAC posreal_ss [Conj_def, One_def, add_sub]
+			    ++ METIS_TAC [])
+		    ++ `(wp (NondetAssign "payer" (zero_to_n_Int_list n))
+       		            (\s. (if n = num_of_value (s "N") then 1 else 0))) =
+	       		    (\s. (if n = num_of_value (s "N") then 1 else 0))`
+			by (`LENGTH (zero_to_n_Int_list n) > 0`
+				by (Cases_on `n`
+		    		    ++ RW_TAC arith_ss [zero_to_n_Int_list, LENGTH_SNOC])
+		    	    ++ `!a s. (\s. (if n = num_of_value (s "N") then (1:posreal) else 0)) s =
+			              (\s. (if n = num_of_value (s "N") then 1 else 0)) 
+			      	      (assign "payer" a s)`
+				by RW_TAC posreal_ss [assign_eta]
+		    	    ++ `!v (l:value list) (e:(string->value)->posreal). (LENGTH l > 0) ==>
+	        		   ((!a s. e s = e (assign v a s)) ==>
+		  	 	   ((wp (NondetAssign v l) e) = e))`
+				by METIS_TAC [NondetAssign_do_nothing_val]
+		    	    ++ FULL_SIMP_TAC std_ss [])
+		    ++ FULL_SIMP_TAC std_ss [])
+	++ RW_TAC posreal_ss [FUN_EQ_THM, One_def]
+	++ MATCH_MP_TAC le_antisym
+	++ `expect1 (\s. (if num_of_value (s "payer") < num_of_value (s "N") then 1 else 0))`
+		by (RW_TAC posreal_ss [expect1_def]
+		    ++ RW_TAC posreal_ss [le_refl, zero_le])
+	++ `expect1 (wp (NondetAssign "payer" (zero_to_n_Int_list n))
+			(\s. (if num_of_value (s "payer") < num_of_value (s "N") then 1 else 0)))`
+		by METIS_TAC [expect1_postE_imp_expect1_wp_postE]
+	++ FULL_SIMP_TAC posreal_ss [expect1_def, Leq_def]
+	++ POP_ASSUM (K ALL_TAC)
+	++ POP_ASSUM (K ALL_TAC)
+	++ Q.ABBREV_TAC `state = (\w. (if w = "NSApays" then No else (if w = "N" then Int (& n) else s w)))`
+	++ `(if n = num_of_value (state "N") then (1:posreal) else 0) <=
+	    wp (NondetAssign "payer" (zero_to_n_Int_list n))
+	       (\s. (if num_of_value (s "payer") < num_of_value (s "N") then 1 else 0)) state`
+		by PROVE_TAC []
+	++ Suff `(1:posreal) <= (if n = num_of_value (state "N") then (1:posreal) else 0)`
+	>> METIS_TAC [le_trans]
+	++ Q.UNABBREV_TAC `state`
+	++ RW_TAC posreal_ss [num_of_value_def, int_of_value_def, NUM_OF_INT],
+	RW_TAC posreal_ss [initialize_def, Program_def, wp_def, set_payer_def, assign_eta, 
+			   initialize_var_NSApays_def, initialize_var_N_def]
+	++ RW_TAC posreal_ss [FUN_EQ_THM, Zero_def]
+	++ `LENGTH (zero_to_n_Int_list n) > 0`
+		by (Cases_on `n`
+		    ++ RW_TAC arith_ss [zero_to_n_Int_list, LENGTH_SNOC])
+	++ `?x y. (MEM x (zero_to_n_Int_list n)) /\ (MEM y (zero_to_n_Int_list n)) /\ (~(x=y))`
+		by (Q.EXISTS_TAC `Int 0`
+		    ++ Q.EXISTS_TAC `Int 1`
+		    ++ RW_TAC int_ss [zero_to_n_Int_list_contains])
+	++ `wp (NondetAssign "payer" (zero_to_n_Int_list n))
+               (\s. (if s "payer" = Int(& k) then 1 else 0)) = Zero`
+		by METIS_TAC [NondetAssign_partial_result]
+	++ RW_TAC posreal_ss [Zero_def],
+	RW_TAC posreal_ss [initialize_def, Program_def, wp_def, set_payer_def, assign_eta, 
+			   initialize_var_NSApays_def, initialize_var_N_def]
+	++ RW_TAC posreal_ss [FUN_EQ_THM, Zero_def]
+	++ `LENGTH (zero_to_n_Int_list n) > 0`
+		by (Cases_on `n`
+		    ++ RW_TAC arith_ss [zero_to_n_Int_list, LENGTH_SNOC])
+	++ `?x y. (MEM x (zero_to_n_Int_list n)) /\ (MEM y (zero_to_n_Int_list n)) /\ (~(x=y))`
+		by (Q.EXISTS_TAC `Int 0`
+		    ++ Q.EXISTS_TAC `Int 1`
+		    ++ RW_TAC int_ss [zero_to_n_Int_list_contains])
+	++ `MEM (Int (& k)) (zero_to_n_Int_list n)`
+		by METIS_TAC [zero_to_n_Int_list_contains]
+	++ `wp (NondetAssign "payer" (zero_to_n_Int_list n))
+	       (\s. (if ~(s "payer" = Int (& k)) then 1 else 0)) = Zero`
+		by METIS_TAC [NondetAssign_result]
+	++ RW_TAC posreal_ss [Zero_def]]]);
+
+val initialize_result2 = store_thm
+  ("initialize_result2",
+   ``!n nsapays k. (n > 0) ==>
+	((wp (initialize n nsapays) (\s. if ((num_of_value (s "N")) = n) then 1 else 0) = One) /\
+	 (wp (initialize n nsapays) (\s. if (s"N" = Int(&n)) then 1 else 0) = One) /\
+	 (wp (initialize n nsapays) (\s. if nsapays 
+					 then (if ((s "NSApays") = Yes) then 1 else 0)								 else (if ((s "NSApays") = No) then 1 else 0)) = One) /\
+	 (if nsapays
+	  then (wp (initialize n nsapays) (\s. if ((s "payer") = (s "N")) then 1 else 0) = One)
+	  else 
+	  ((wp (initialize n nsapays) 
+	       (\s. if ((num_of_value (s "payer")) < 
+		        (num_of_value (s "N"))) then 1 else 0) = One)
+	    /\ ((n > 1) ==> ((wp (initialize n nsapays)
+			         (\s. if (s "payer") = Int (& k) then 1 else 0) = Zero)
+	    		     /\ ( (k < n) ==>
+				(wp (initialize n nsapays)
+				    (\s. if ~ ((s "payer") = Int (& k)) 
+					 then 1 else 0) = Zero)))))))``,
+    RW_TAC bool_ss [FORALL_AND_THM, initialize_result]
+    ++ RW_TAC std_ss [initialize_def, Program_def, wp_def, set_payer_def, 
+		   initialize_var_NSApays_def, assign_eta]
+    >> RW_TAC posreal_ss [initialize_var_N_result2]
+    ++ `wp (NondetAssign "payer" (zero_to_n_Int_list n))
+	   (\s. (if s "N" = Int (& n) then 1 else 0)) =
+	   (\s. (if s "N" = Int (& n) then 1 else 0))`
+	by (`LENGTH (zero_to_n_Int_list n) > 0`
+		by (Cases_on `n`
+	    	    ++ RW_TAC arith_ss [zero_to_n_Int_list, LENGTH_SNOC])
+	    ++ `!(n:num). (n > 0) ==>
+		(?(l:value list). l = zero_to_n_Int_list n)`
+		by (Induct_on `n`
+	    	    ++ RW_TAC arith_ss [])
+	    ++ `?l. zero_to_n_Int_list n = l` by METIS_TAC []
+	    ++ `LENGTH l > 0` by RW_TAC arith_ss []
+	    ++ ASM_REWRITE_TAC []
+	    ++ `!a s. (\s. (if s "N" = Int (& n) then (1:posreal) else 0)) s =
+		      (\s. (if s "N" = Int (& n) then 1 else 0))
+		      (assign "payer" a s)` 
+		by RW_TAC std_ss [assign_eta]
+	    ++ `!(v :string) (l :value list) (e :(string -> value) -> posreal).
+         	 LENGTH l > (0 :num) ==>
+         	 (!(a :(string -> value) -> value) (s :string -> value).
+          	 e s = e (assign v a s)) ==>
+         	(wp (NondetAssign v l) e = e)` 
+		by METIS_TAC [NondetAssign_do_nothing_val]
+	    ++ FULL_SIMP_TAC std_ss [])
+    ++ RW_TAC std_ss [initialize_var_N_result2]);
+
+(* -------------------------- flip_coins proofs ---------------------------- *)
+
+val flip_coins_term = store_thm
+  ("flip_coins_term",
+   ``!n nsapays k. (n > 0) ==>
+	(wp (Seq (initialize n nsapays) (flip_coins)) One = One)``,
+   REPEAT STRIP_TAC
+   ++ MATCH_MP_TAC seq_term
+   ++ RW_TAC std_ss [initialize_term, flip_coins_def, Program_def, wp_def]
+   ++ `wp (For_0_to_n "i" "N"
+		      [ProbAssign "coinflip" [Heads; Tails];
+		       Assign_Array_i "Coins" "i" (\s. s "coinflip")]) One = One`
+	by (`~("N" = "i")` by SRW_TAC [] []
+	    ++ `Leq (\s. if (\s. (0 <= int_of_value (s "i"))) s then 1 else 0)
+		    (wp (Program
+			 [ProbAssign "coinflip" [Heads; Tails];
+			  Assign_Array_i "Coins" "i" (\s. s "coinflip")])
+			(\s. if (\s. (0 <= int_of_value (s "i"))) s then 1 else 0))`
+		by (SRW_TAC [] [Program_def, wp_def, Assign_Array_i_def, assign_eta]
+		    ++ Suff `wp (ProbAssign "coinflip" [Heads; Tails])
+		                (\s. (if 0 <= int_of_value (s "i") then (1:posreal) else 0)) = 
+			        (\s. (if 0 <= int_of_value (s "i") then (1:posreal) else 0))`
+		    >> (RW_TAC std_ss [] ++ METIS_TAC [leq_refl])
+		    ++ `!v l e. (LENGTH l > 0) ==>
+	        ((!a (s:string->value). e s = e (assign v a s)) ==>
+		   ((wp (ProbAssign v l) e) = e))` by METIS_TAC [ProbAssign_do_nothing_val]
+		    ++ `!a s. (\s. (if 0 <= int_of_value (s "i") then (1:posreal) else 0)) s =
+			      (\s. (if 0 <= int_of_value (s "i") then 1 else 0))
+			      (assign "coinflip" a s)` 
+			by SRW_TAC [] [assign_eta]
+		    ++ `LENGTH [Heads;Tails] > 0` by RW_TAC arith_ss [LENGTH]
+		    ++ FULL_SIMP_TAC std_ss [])
+	    ++ `!N. Leq (\s. if (\s.((int_of_value (s "i")) < (int_of_value (s "N")))) s /\
+			        (\s.(0 <= (int_of_value(s "i")))) s /\
+			        ((\s.((int_of_value (s "N")) - (int_of_value (s "i")))) s = N)
+			     then 1 else 0)
+			(wp (Program
+			     [ProbAssign "coinflip" [Heads; Tails];
+			      Assign_Array_i "Coins" "i" (\s. s "coinflip")])
+			    (\s. if ((\s.((int_of_value (s "N")) - (int_of_value (s "i")))) s <= N) 
+			         then 1 else 0))`
+		by (SRW_TAC [] [Program_def, wp_def, Assign_Array_i_def, assign_eta]
+		    ++ `Leq (\s. (if int_of_value (s "i") < int_of_value (s "N") /\
+				     0 <= int_of_value (s "i") /\
+				     (int_of_value (s "N") - int_of_value (s "i") = N)
+				  then 1 else 0))
+			    (\s. (if int_of_value (s "N") - int_of_value (s "i") <= N 
+				  then 1 else 0))`
+			by (RW_TAC posreal_ss [Leq_def]
+			    ++ RW_TAC posreal_ss []
+			    ++ METIS_TAC [INT_LE_REFL])
+		    ++ Suff `(wp (ProbAssign "coinflip" [Heads; Tails])
+				 (\s. (if int_of_value (s "N") - int_of_value (s "i") <= N 
+				       then 1 else 0))) =
+			     (\s. (if int_of_value (s "N") - int_of_value (s "i") <= N 
+				  then 1 else 0))`
+		    >> (RW_TAC std_ss [] ++ METIS_TAC [leq_trans])
+		    ++ `!v l e. (LENGTH l > 0) ==>
+	        ((!a (s:string->value). e s = e (assign v a s)) ==>
+		   ((wp (ProbAssign v l) e) = e))` by METIS_TAC [ProbAssign_do_nothing_val]
+		    ++ `!a s. (\s. (if int_of_value (s "N") - 
+				       int_of_value (s "i") <= N then (1:posreal) else 0)) s =
+			      (\s. (if int_of_value (s "N") - 
+				       int_of_value (s "i") <= N then 1 else 0))
+			      (assign "coinflip" a s)` 
+			by SRW_TAC [] [assign_eta]
+		    ++ `LENGTH [Heads;Tails] > 0` by RW_TAC arith_ss [LENGTH]
+		    ++ FULL_SIMP_TAC std_ss [])
+	    ++ METIS_TAC [For_i_0_to_n_variant_rule])
+	++ RW_TAC std_ss [New_Array_def, wp_def, assign_eta, One_def]);
+
+val flip_coins_result_part1 = store_thm
+  ("flip_coins_result_part1",
+   ``!(n :num) (nsapays :bool) (i :num).
+      n > (0 :num) /\ i < n ==>
+      (wp (Seq (initialize n nsapays) flip_coins)
+         (\(s :value state).
+            (if
+               (get_Array_i (s "Coins") i = Heads) \/
+               (get_Array_i (s "Coins") i = Tails)
+             then
+               (1 :
+             posreal)
+             else
+               (0 :
+             posreal))) =
+       (One :value state expect))``,
+   RW_TAC std_ss [wp_def]
+   ++ MATCH_MP_TAC leq_antisym
+       ++ `Leq
+      (wp (initialize (n :num) (nsapays :bool))
+         (wp flip_coins
+            (\(s :value state).
+               (if
+                  (get_Array_i (s "Coins") (i :num) = Heads) \/
+                  (get_Array_i (s "Coins") i = Tails)
+                then
+                  (1 :
+                posreal)
+                else
+                  (0 :
+                posreal))))) (One :value state expect)`
+	by (`Leq
+      (wp flip_coins
+         (\(s :value state).
+            (if
+               (get_Array_i (s "Coins") (i :num) = Heads) \/
+               (get_Array_i (s "Coins") i = Tails)
+             then
+               (1 :
+             posreal)
+             else
+               (0 :
+             posreal)))) (One :value state expect)`
+		by (`expect1
+      (\(s :value state).
+         (if
+            (get_Array_i (s "Coins") (i :num) = Heads) \/
+            (get_Array_i (s "Coins") i = Tails)
+          then
+            (1 :
+          posreal)
+          else
+            (0 :
+          posreal)))`
+			by (RW_TAC posreal_ss [expect1_def]
+		    	    ++ RW_TAC posreal_ss [le_refl, zero_le])
+       		    ++ `expect1
+      (wp flip_coins
+         (\(s :value state).
+            (if
+               (get_Array_i (s "Coins") (i :num) = Heads) \/
+               (get_Array_i (s "Coins") i = Tails)
+             then
+               (1 :
+             posreal)
+             else
+               (0 :
+             posreal))))`
+			by METIS_TAC [expect1_postE_imp_expect1_wp_postE]
+       		    ++ FULL_SIMP_TAC posreal_ss [expect1_def, Leq_def, One_def]
+		    ++ RW_TAC std_ss [])
+	    ++ `expect1
+      (wp flip_coins
+         (\(s :value state).
+            (if
+               (get_Array_i (s "Coins") (i :num) = Heads) \/
+               (get_Array_i (s "Coins") i = Tails)
+             then
+               (1 :
+             posreal)
+             else
+               (0 :
+             posreal))))`
+		by FULL_SIMP_TAC posreal_ss [expect1_def, Leq_def, One_def]
+	    ++ `expect1
+      (wp (initialize (n :num) (nsapays :bool))
+         (wp flip_coins
+            (\(s :value state).
+               (if
+                  (get_Array_i (s "Coins") (i :num) = Heads) \/
+                  (get_Array_i (s "Coins") i = Tails)
+                then
+                  (1 :
+                posreal)
+                else
+                  (0 :
+                posreal)))))`
+		by METIS_TAC [expect1_postE_imp_expect1_wp_postE]
+	    ++ FULL_SIMP_TAC posreal_ss [expect1_def, Leq_def, One_def])
+        ++ ASM_REWRITE_TAC []
+	++ POP_ASSUM (K ALL_TAC)
+	++ RW_TAC posreal_ss [flip_coins_def, For_0_to_n_def, wp_def, Program_def]
+	++ RW_TAC std_ss [For_def]
+	++ `wp
+      (Seq (Assign "i" (\(s :value state). Int (0 :int)))
+         (While
+            (\(s :value state). int_of_value (s "i") < int_of_value (s "N"))
+            (Seq
+               (Program
+                  [ProbAssign "coinflip" [Heads; Tails];
+                   Assign_Array_i "Coins" "i"
+                     (\(s :value state). s "coinflip")])
+               (Assign "i"
+                  (\(s :value state).
+                     Int (int_of_value (s "i") + (1 :int)))))))
+      (\(s :value state).
+         (if
+            (get_Array_i (s "Coins") (i :num) = Heads) \/
+            (get_Array_i (s "Coins") i = Tails)
+          then
+            (1 :
+          posreal)
+          else
+            (0 :
+          posreal))) =
+    wp (Assign "i" (\(s :value state). Int (0 :int)))
+      (wp
+         (While
+            (\(s :value state). int_of_value (s "i") < int_of_value (s "N"))
+            (Seq
+               (Program
+                  [ProbAssign "coinflip" [Heads; Tails];
+                   Assign_Array_i "Coins" "i"
+                     (\(s :value state). s "coinflip")])
+               (Assign "i"
+                  (\(s :value state).
+                     Int (int_of_value (s "i") + (1 :int))))))
+         (\(s :value state).
+            (if
+               (get_Array_i (s "Coins") i = Heads) \/
+               (get_Array_i (s "Coins") i = Tails)
+             then
+               (1 :
+             posreal)
+             else
+               (0 :
+             posreal))))`
+		by METIS_TAC [wp_def]
+	++ ASM_REWRITE_TAC []
+	++ POP_ASSUM (K ALL_TAC)
+	++ Q.ABBREV_TAC `Inv = (\(v :num) (s :value state).
+                (v = num_of_value (s "N") - num_of_value (s "i")) /\
+                (0 :int) <= int_of_value (s "i") /\
+                v <= num_of_value (s "N") /\
+                int_of_value (s "i") <= int_of_value (s "N") /\
+                (!(j :num).
+                   j < num_of_value (s "i") ==>
+                   (get_Array_i (s "Coins") j = Heads) \/
+                   (get_Array_i (s "Coins") j = Tails)) /\
+                (?(l :value list). s "Coins" = Array l) /\
+                (Array_length (s "Coins") = num_of_value (s "N")) /\
+                (num_of_value (s "N") = (n :num)) /\
+                (s "N" = Int (& n :int)))`
+	++ Q.ABBREV_TAC `body = Seq
+               (Program
+                  [ProbAssign "coinflip" [Heads; Tails];
+                   Assign_Array_i "Coins" "i"
+                     (\(s :value state). s "coinflip")])
+               (Assign "i"
+                  (\(s :value state).
+                     Int (int_of_value (s "i") + (1 :int))))`
+	++ Q.ABBREV_TAC `g = (\(s :value state).
+                int_of_value (s "i") < int_of_value (s "N"))`
+	++ `!v:num. Leq (bool_exp (Inv v))
+			(wp (While g body)
+			    (bool_exp (\s. ?v'. Inv v' s /\ (~(g s)))))`
+		by (MATCH_MP_TAC bool_Inv_rule
+		    ++ GEN_TAC
+		    ++ RW_TAC posreal_ss [bool_exp_def, Leq_def]
+		    ++ RW_TAC posreal_ss [zero_le]
+		    ++ Q.UNABBREV_TAC `body`
+		    ++ RW_TAC posreal_ss [Program_def, wp_def, assign_eta, Assign_Array_i_def, 
+					  ProbAssign_def, MAP, Probs_def, LENGTH]
+		    ++ Q.UNABBREV_TAC `Inv`
+		    ++ Q.UNABBREV_TAC `g`
+		    ++ `(\(v :value state).
+       (1 :posreal) / (2 :posreal) /
+       ((1 :posreal) - (1 :posreal) / (2 :posreal))) =
+    (\(v :value state). (1 :posreal))`
+			by (RW_TAC posreal_ss [FUN_EQ_THM, sub_ratr, div_rat, preal_div_def]
+			    ++ MATCH_MP_TAC mul_linv
+			    ++ RW_TAC posreal_ss [])
+		    ++ ASM_REWRITE_TAC []
+		    ++ POP_ASSUM (K ALL_TAC)
+		    ++ FULL_SIMP_TAC posreal_ss [lin_eta, bound1_def, mul_lone, Zero_def, mul_rzero, 
+						 int_of_value_def, let_lemma, let_lin_lemma]
+		    ++ `(0 :int) <= int_of_value ((s :value state) "i") + (1 :int)`
+			by RW_TAC int_ss []
+		    ++ `~("Coins" = "i")` by SRW_TAC [] []
+		    ++ `~("N" = "i")` by SRW_TAC [] []
+		    ++ `~("N" = "Coins")` by SRW_TAC [] []
+		    ++ `~("N" = "coinflip")` by SRW_TAC [] []
+		    ++ FULL_SIMP_TAC std_ss [num_of_value_def, int_of_value_def]
+		    ++ POP_ASSUM (K ALL_TAC)
+		    ++ POP_ASSUM (K ALL_TAC)
+		    ++ POP_ASSUM (K ALL_TAC)
+		    ++ POP_ASSUM (K ALL_TAC)
+		    ++ `(0 :int) <= (& (n :num) :int)`
+			 by (MATCH_MP_TAC INT_LT_IMP_LE 
+			     ++ METIS_TAC [INT_LET_TRANS])
+   		    ++ `?(n' :num). int_of_value ((s :value state) "N") = (& n' :int)`
+			by METIS_TAC [int_of_value_def]
+		    ++ `?(i' :num). int_of_value ((s :value state) "i") = (& i' :int)`
+			by METIS_TAC [NUM_POSINT_EXISTS]
+		    ++ `(& (i' :num) :int) + (1 :int) = (& (SUC i') :int)` by METIS_TAC [INT]
+		    ++ FULL_SIMP_TAC int_ss [NUM_OF_INT]
+		    ++ Suff `((!(j :num).
+        j < SUC (i' :num) ==>
+        (get_Array_i (update_Array_i (Array (l :value list)) i' Heads) j =
+         Heads) \/
+        (get_Array_i (update_Array_i (Array l) i' Heads) j = Tails)) /\
+     (?(l' :value list). update_Array_i (Array l) i' Heads = Array l') /\
+     (Array_length (update_Array_i (Array l) i' Heads) = (n :num))) /\
+    (!(j :num).
+       j < SUC i' ==>
+       (get_Array_i (update_Array_i (Array l) i' Tails) j = Heads) \/
+       (get_Array_i (update_Array_i (Array l) i' Tails) j = Tails)) /\
+    (?(l' :value list). update_Array_i (Array l) i' Tails = Array l') /\
+    (Array_length (update_Array_i (Array l) i' Tails) = n)`
+		    >> (RW_TAC posreal_ss [sub_ratr, add_rat]
+			++ RW_TAC posreal_ss [preal_div_def]
+			++ Suff `(4 :posreal) * inv (4 :posreal) = (1 :posreal)`
+			>> METIS_TAC [le_refl]
+			++ MATCH_MP_TAC mul_rinv
+		        ++ RW_TAC posreal_ss [])
+		    ++ `(0 :num) < (n :num) - (i' :num)`
+			by (`!(a :num) (b :num). a < b ==> (0 :num) < b - a` by RW_TAC arith_ss []
+		    	    ++ METIS_TAC [])
+		    ++ `Array_length (update_Array_i (Array (l :value list)) (i' :num) Tails) =
+    Array_length ((s :value state) "Coins")`
+			by (`?(l' :value list).
+      update_Array_i (Array (l :value list)) (i' :num) Tails = Array l'`
+				by RW_TAC std_ss [update_Array_i_def]
+		    	    ++ METIS_TAC [update_Array_i_length])
+		    ++ `Array_length (update_Array_i (Array (l :value list)) (i' :num) Heads) =
+    Array_length ((s :value state) "Coins")`
+			by (`?(l' :value list).
+      update_Array_i (Array (l :value list)) (i' :num) Heads = Array l'`
+				by RW_TAC std_ss [update_Array_i_def]
+		    	    ++ METIS_TAC [update_Array_i_length])
+		    ++ `(!(j :num).
+       j < SUC (i' :num) ==>
+       (get_Array_i (update_Array_i (Array (l :value list)) i' Heads) j =
+        Heads) \/
+       (get_Array_i (update_Array_i (Array l) i' Heads) j = Tails)) /\
+    (?(l' :value list). update_Array_i (Array l) i' Heads = Array l') =
+    !(j :num).
+      j < SUC i' ==>
+      (get_Array_i (update_Array_i (Array l) i' Heads) j = Heads) \/
+      (get_Array_i (update_Array_i (Array l) i' Heads) j = Tails)`
+			by RW_TAC std_ss [update_Array_i_def]
+		    ++ `(!(j :num).
+       j < SUC (i' :num) ==>
+       (get_Array_i (update_Array_i (Array (l :value list)) i' Tails) j =
+        Heads) \/
+       (get_Array_i (update_Array_i (Array l) i' Tails) j = Tails)) /\
+    (?(l' :value list). update_Array_i (Array l) i' Tails = Array l') =
+    !(j :num).
+      j < SUC i' ==>
+      (get_Array_i (update_Array_i (Array l) i' Tails) j = Heads) \/
+      (get_Array_i (update_Array_i (Array l) i' Tails) j = Tails)`
+			by RW_TAC std_ss [update_Array_i_def]
+		    ++ FULL_SIMP_TAC std_ss []
+		    ++ POP_ASSUM (K ALL_TAC)
+		    ++ POP_ASSUM (K ALL_TAC)
+		    ++ `!(j :num).
+      j < SUC (i' :num) ==>
+      (get_Array_i (update_Array_i (Array (l :value list)) i' Heads) j =
+       Heads) \/ (get_Array_i (update_Array_i (Array l) i' Heads) j = Tails)`
+			by (REPEAT STRIP_TAC
+		    	    ++ `(j :num) <= (i' :num)` by RW_TAC int_ss []
+		    	    ++ `(j :num) < Array_length ((s :value state) "Coins")`
+				by METIS_TAC [LESS_EQ_LESS_TRANS]
+		    	    ++ `get_Array_i (update_Array_i (Array (l :value list)) (i' :num) Heads)
+      (j :num) =
+    (if j = i' then Heads else get_Array_i (Array l) j)`
+				by METIS_TAC [update_Array_i_el]
+		    	    ++ ASM_REWRITE_TAC []
+		    	    ++ Cases_on `j = i'`
+		    	    >> RW_TAC std_ss []
+		    	    ++ `(j :num) < (i' :num)` by RW_TAC int_ss []
+		    	    ++ METIS_TAC [])
+		    ++ `!(j :num).
+      j < SUC (i' :num) ==>
+      (get_Array_i (update_Array_i (Array (l :value list)) i' Tails) j =
+       Heads) \/ (get_Array_i (update_Array_i (Array l) i' Tails) j = Tails)`
+			by (REPEAT STRIP_TAC
+		    	    ++ `(j :num) <= (i' :num)` by RW_TAC int_ss []
+		    	    ++ `(j :num) < Array_length ((s :value state) "Coins")`
+				by METIS_TAC [LESS_EQ_LESS_TRANS]
+		    	    ++ `get_Array_i (update_Array_i (Array (l :value list)) (i' :num) Tails)
+      (j :num) =
+    (if j = i' then Tails else get_Array_i (Array l) j)`
+				by METIS_TAC [update_Array_i_el]
+		    	    ++ ASM_REWRITE_TAC []
+		    	    ++ Cases_on `j = i'`
+		    	    >> RW_TAC std_ss []
+		    	    ++ `(j :num) < (i' :num)` by RW_TAC int_ss []
+		    	    ++ METIS_TAC [])
+		    ++ RW_TAC std_ss [])
+	++ `Leq (bool_exp ((Inv :num -> value state -> bool) (n :num)))
+      (wp (While (g :value state -> bool) (body :value command))
+         (\(s :value state).
+            (if
+               (get_Array_i (s "Coins") (i :num) = Heads) \/
+               (get_Array_i (s "Coins") i = Tails)
+             then
+               (1 :
+             posreal)
+             else
+               (0 :
+             posreal))))`
+		by (`Leq
+      (wp (While (g :value state -> bool) (body :value command))
+         (bool_exp
+            (\(s :value state).
+               ?(v' :num). (Inv :num -> value state -> bool) v' s /\ ~g s)))
+      (wp (While g body)
+         (\(s :value state).
+            (if
+               (get_Array_i (s "Coins") (i :num) = Heads) \/
+               (get_Array_i (s "Coins") i = Tails)
+             then
+               (1 :
+             posreal)
+             else
+               (0 :
+             posreal))))`
+			by (`Leq
+      (bool_exp
+         (\(s :value state).
+            ?(v' :num).
+              (Inv :num -> value state -> bool) v' s /\
+              ~(g :value state -> bool) s))
+      (\(s :value state).
+         (if
+            (get_Array_i (s "Coins") (i :num) = Heads) \/
+            (get_Array_i (s "Coins") i = Tails)
+          then
+            (1 :
+          posreal)
+          else
+            (0 :
+          posreal)))`
+				by (POP_ASSUM (K ALL_TAC)
+				    ++ RW_TAC posreal_ss [Leq_def, bool_exp_def]
+				    ++ Suff `(?(v' :num).
+       (Inv :num -> value state -> bool) v' (s :value state) /\
+       ~(g :value state -> bool) s) ==>
+    (get_Array_i (s "Coins") (i :num) = Heads) \/
+    (get_Array_i (s "Coins") i = Tails)`
+			    	    >> RW_TAC posreal_ss [zero_le, le_refl]
+			  	    ++ Q.UNABBREV_TAC `Inv`
+				    ++ Q.UNABBREV_TAC `g`
+				    ++ RW_TAC std_ss []
+				    ++ `int_of_value ((s :value state) "i") = int_of_value (s "N")`
+					by (FULL_SIMP_TAC int_ss [INT_NOT_LT]
+					    ++ METIS_TAC [INT_LE_ANTISYM])
+		  		    ++ FULL_SIMP_TAC std_ss [num_of_value_def])
+		 	   ++ METIS_TAC [wp_mono])
+		    ++ METIS_TAC [leq_trans])
+	++ Suff `Leq (One :value state expect)
+      (wp (initialize (n :num) (nsapays :bool))
+         (wp (New_Array "Coins" "N")
+            (wp (Assign "i" (\(s :value state). Int (0 :int)))
+               (bool_exp ((Inv :num -> value state -> bool) n)))))`
+	>> PROVE_TAC [wp_mono, leq_trans]
+	++ POP_ASSUM (K ALL_TAC)
+	++ POP_ASSUM (K ALL_TAC)
+	++ Q.UNABBREV_TAC `body`
+	++ Q.UNABBREV_TAC `g`
+	++ Q.UNABBREV_TAC `Inv`
+	++ SRW_TAC [] [bool_exp_def, wp_def, assign_eta, New_Array_def, 
+		       num_of_value_def, int_of_value_def, Array_length_def]
+	++ `(\(s :value state).
+       (if
+          ((n :num) = Num (int_of_value (s "N"))) /\
+          n <= Num (int_of_value (s "N")) /\
+          (0 :int) <= int_of_value (s "N") /\
+          (LENGTH (n_list (Num (int_of_value (s "N"))) Null) =
+           Num (int_of_value (s "N"))) /\
+          (Num (int_of_value (s "N")) = n) /\ (s "N" = Int (& n :int))
+        then
+          (1 :
+        posreal)
+        else
+          (0 :
+        posreal))) =
+    (\(s :value state).
+       (if (s "N" = Int (& n :int)) /\ (Num (int_of_value (s "N")) = n) then
+          (1 :
+        posreal)
+        else
+          (0 :
+        posreal)))`
+		by (RW_TAC std_ss [FUN_EQ_THM]
+		    ++ RW_TAC posreal_ss []
+		    >> (FULL_SIMP_TAC arith_ss [int_of_value_def]
+			++ `~((0 :int) <= (& (Num (int_of_value ((s :value state) "N"))) :int))` by METIS_TAC [int_of_value_def]
+			++ FULL_SIMP_TAC int_ss [INT_LE_REDUCE])
+		    ++ FULL_SIMP_TAC arith_ss [int_of_value_def, length_of_n_list])
+	++ ASM_REWRITE_TAC []
+	++ POP_ASSUM (K ALL_TAC)
+	++ `(\(s :value state).
+       (if
+          (s "N" = Int (& (n :num) :int)) /\
+          (Num (int_of_value (s "N")) = n)
+        then
+          (1 :
+        posreal)
+        else
+          (0 :
+        posreal))) =
+    Conj
+      (\(s :value state).
+         (if s "N" = Int (& n :int) then (1 :posreal) else (0 :posreal)))
+      (\(s :value state).
+         (if Num (int_of_value (s "N")) = n then
+            (1 :
+          posreal)
+          else
+            (0 :
+          posreal)))`
+		by (RW_TAC posreal_ss [Conj_def, FUN_EQ_THM]
+		    ++ RW_TAC posreal_ss [])
+	++ ASM_REWRITE_TAC []
+	++ POP_ASSUM (K ALL_TAC)
+	++ Suff `(One :value state expect) =
+    Conj
+      (wp (initialize (n :num) (nsapays :bool))
+         (\(s :value state).
+            (if s "N" = Int (& n :int) then
+               (1 :
+             posreal)
+             else
+               (0 :
+             posreal))))
+      (wp (initialize n nsapays)
+         (\(s :value state).
+            (if Num (int_of_value (s "N")) = n then
+               (1 :
+             posreal)
+             else
+               (0 :
+             posreal))))`
+	>> PROVE_TAC [leq_trans, leq_refl, wp_conj]
+	++ `wp (initialize (n :num) (nsapays :bool))
+      (\(s :value state).
+         (if s "N" = Int (& n :int) then (1 :posreal) else (0 :posreal))) =
+    (One :value state expect)`
+		by METIS_TAC [initialize_result2]
+	++ ASM_REWRITE_TAC []
+	++ POP_ASSUM (K ALL_TAC)
+	++ `wp (initialize (n :num) (nsapays :bool))
+      (\(s :value state).
+         (if num_of_value (s "N") = n then
+            (1 :
+          posreal)
+          else
+            (0 :
+          posreal))) =
+    (One :value state expect)`
+		by METIS_TAC [initialize_result2, num_of_value_def]
+	++ FULL_SIMP_TAC std_ss [num_of_value_def]
+	++ POP_ASSUM (K ALL_TAC)
+	++ RW_TAC posreal_ss [Conj_def, One_def]);
+
+(* ???????????????????????????????????????????????
+
+val flip_coins_result = store_thm
+  ("flip_coins_result",
+   ``!n nsapays i. (n > 0) /\
+	(i < n) ==>
+	(wp (Seq (initialize n nsapays) (flip_coins))
+	   (\s. if ((get_Array_i (s "Coins") i) = Heads) \/
+		   ((get_Array_i (s "Coins") i) = Tails)
+		then 1 else 0) = 
+	 One) /\
+	(wp (Seq (initialize n nsapays) (flip_coins))
+	    (\s. if ((get_Array_i (s "Coins") i) = Heads)
+		 then 1 else 0) =
+	 (\s. 1/2)) /\
+	(wp (Seq (initialize n nsapays) (flip_coins))
+	    (\s. if ((get_Array_i (s "Coins") i) = Tails)
+		 then 1 else 0) =
+	 (\s. 1/2))``,
+   REPEAT STRIP_TAC
+   << [METIS_TAC [flip_coins_result_part1],
+       METIS_TAC [flip_coins_result_part2],
+       METIS_TAC [flip_coins_result_part3]]);
+
+??????????????????????????????????????????????? *)
+
+(* ----------------------- set_announcements proofs ------------------------ *)
 
 val set_announcements_term = store_thm
   ("set_announcements_term",
-   ``((wp set_announcements One) (\s. if ((s"N" = 0) \/ (s"N" > 0)) then 1 else 0)) = 1``,
-   ????);
+   ``!n nsapays. (n > 0) ==>
+	(wp (Program [initialize n nsapays; flip_coins; set_announcements]) One = One)``,
+	REPEAT STRIP_TAC
+	++ `wp (Program [initialize n nsapays; flip_coins; set_announcements]) One =
+	    wp (Seq (initialize n nsapays) (flip_coins)) (wp set_announcements One)`
+		by METIS_TAC [Program_def, wp_def, seq_assoc]
+	++ ASM_REWRITE_TAC []
+	++ POP_ASSUM (K ALL_TAC)
+	++ Suff `wp set_announcements One = One`
+	>> METIS_TAC [flip_coins_term]
+	++ SIMP_TAC std_ss [set_announcements_def, Program_def, wp_def]
+	++ `wp (New_Array "Announces" "N") One = One`
+		by RW_TAC posreal_ss [New_Array_def, wp_def, assign_eta, One_def]
+	++ Suff `(wp (For_0_to_n "i" "N"
+            		[Assign "currentcoin"
+               			(\s. get_Array_i (s "Coins") (num_of_value (s "i")));
+             		If (\s. num_of_value (s "i") = 0)
+               			(Assign "previouscoin"
+                  			(\s. get_Array_i (s "Coins") (num_of_value (s "N") - 1)))
+               			(Assign "previouscoin"
+                  			(\s. get_Array_i (s "Coins") (num_of_value (s "i") - 1)));
+             		If (\s. s "i" = s "payer") (Assign "pays" (\s. Yes))
+               			(Assign "pays" (\s. No));
+             		Assign_Array_i "Announces" "i"
+               			(\s. xor [s "previouscoin"; s "currentcoin"; s "pays"])]) One) = One`
+	>> RW_TAC std_ss []
+	++ POP_ASSUM (K ALL_TAC)
+	++ MATCH_MP_TAC For_i_0_to_n_variant_rule
+	++ SRW_TAC [] []
+	>> (RW_TAC std_ss [Program_def, wp_def, assign_eta, If_def, lin_eta, Leq_def, Assign_Array_i_def]
+	    ++ `~((if 0 <= int_of_value (s "i") then 1 else 0) = infty)`
+			by RW_TAC posreal_ss []
+	    ++ Q.UNABBREV_TAC `x'`
+	    ++ `((bound1 (if s "i" = s "payer" then 1 else 0)) * 
+		(if 0 <= int_of_value (s "i") then 1 else 0) +
+		(1 - (bound1 (if s "i" = s "payer" then 1 else 0))) * 
+		(if 0 <= int_of_value (s "i") then 1 else 0)) =
+		(if 0 <= int_of_value (s "i") then 1 else 0)`
+			by PROVE_TAC [bound1_eq_lemma]
+	    ++ ASM_REWRITE_TAC []
+	    ++ POP_ASSUM (K ALL_TAC)
+	    ++ Q.UNABBREV_TAC `x`
+	    ++ PROVE_TAC [bound1_eq_lemma, le_refl])
+	++ `Leq (\s. (if int_of_value (s "i") < int_of_value (s "N") /\
+				     0 <= int_of_value (s "i") /\
+				     (int_of_value (s "N") - int_of_value (s "i") = N)
+				  then 1 else 0))
+			    (\s. (if int_of_value (s "N") - int_of_value (s "i") <= N 
+				  then 1 else 0))`
+			by (RW_TAC posreal_ss [Leq_def]
+			    ++ RW_TAC posreal_ss []
+			    ++ METIS_TAC [INT_LE_REFL])
+	++ Suff `(wp (Program
+            		[Assign "currentcoin"
+               			(\s. get_Array_i (s "Coins") (num_of_value (s "i")));
+             		If (\s. num_of_value (s "i") = 0)
+               			(Assign "previouscoin"
+                  			(\s. get_Array_i (s "Coins") (num_of_value (s "N") - 1)))
+               			(Assign "previouscoin"
+                  			(\s. get_Array_i (s "Coins") (num_of_value (s "i") - 1)));
+             		If (\s. s "i" = s "payer") (Assign "pays" (\s. Yes))
+               			(Assign "pays" (\s. No));
+             		Assign_Array_i "Announces" "i"
+               			(\s. xor [s "previouscoin"; s "currentcoin"; s "pays"])])
+         	(\s. (if int_of_value (s "N") - int_of_value (s "i") <= N then 1 else 0))) =
+		(\s. (if int_of_value (s "N") - int_of_value (s "i") <= N then 1 else 0))`
+	>> (RW_TAC std_ss [] ++ METIS_TAC [leq_trans])
+	++ RW_TAC std_ss [Program_def, wp_def, assign_eta, If_def, lin_eta, Assign_Array_i_def, FUN_EQ_THM]
+	++ `~((if int_of_value (s "N") - int_of_value (s "i") <= N then 1 else 0) = infty)`
+		by RW_TAC posreal_ss []
+	++ Q.UNABBREV_TAC `x'`
+	++ `((bound1 (if s "i" = s "payer" then 1 else 0)) * 
+		(if int_of_value (s "N") - int_of_value (s "i") <= N then 1 else 0) +
+		(1 - (bound1 (if s "i" = s "payer" then 1 else 0))) * 
+		(if int_of_value (s "N") - int_of_value (s "i") <= N then 1 else 0)) =
+		(if int_of_value (s "N") - int_of_value (s "i") <= N then 1 else 0)`
+			by PROVE_TAC [bound1_eq_lemma]
+	++ ASM_REWRITE_TAC []
+	++ POP_ASSUM (K ALL_TAC)
+	++ Q.UNABBREV_TAC `x`
+	++ PROVE_TAC [bound1_eq_lemma]);
+
+(* ???????????????????????????????????????????????
 
 val set_announcements_result = store_thm
-  ("set_announcements_result",
-   ``!k. ((k>0) \/ (k=0)) ==>
-	((((wp set_announcements (\s. if (((get_Array_i (s"Coins") k) = Heads) \/   
-					  ((get_Array_i (s"Coins") k) = Heads)) then 1 else 0))
-	  (\s. if ((k<s"N")\/(k=s"N")) then 1 else 0)) = 1) /\
-	(((wp set_announcements (\s. if ((get_Array_i (s"Coins") k) = Heads) then 1 else 0))
-	  (\s. if ((k<s"N")\/(k=s"N")) then 1 else 0)) = 0.5) /\
-	(((wp set_announcements (\s. if ((get_Array_i (s"Coins") k) = Tails) then 1 else 0))
-	  (\s. if ((k<s"N")\/(k=s"N")) then 1 else 0)) = 0.5))``,
+   ("set_announcements_result",
+   ``!n nsapays i.
+     (i < n) ==>
+	wp (Program [initialize n nsapays; flip_coins; set_announcements])
+	   (\s. let a = (get_Array_i (s "Announces") i) in
+		if i = (s "payer")
+		then
+		   (let p = Yes in
+		    if i = 0
+		    then
+			(let (c1, c2) = (get_Array_i (s "Coins") 0, get_Array_i (s "Coins") n - 1) in
+			 if a = (xor [p; c1; c2]) then 1 else 0)
+		    else
+		    	(let (c1, c2) = (get_Array_i (s "Coins") i, get_Array_i (s "Coins") i - 1) in
+			 if a = (xor [p; c1; c2]) then 1 else 0))
+		else
+		   (let p = No in
+		    if i = 0
+		    then
+			(let (c1, c2) = (get_Array_i (s "Coins") 0, get_Array_i (s "Coins") n - 1) in
+			 if a = (xor [p; c1; c2]) then 1 else 0)
+		    else
+		    	(let (c1, c2) = (get_Array_i (s "Coins") i, get_Array_i (s "Coins") i - 1) in
+			 if a = (xor [p; c1; c2]) then 1 else 0))) = One``,
+   ???);
+
+??????????????????????????????????????????????? *)
+
+(* ------------------------- compute_result proofs ------------------------- *)
+
+val compute_result_term = store_thm
+  ("compute_result_term",
+   ``!n nsapays. (n>0) ==>
+	(wp (Program [initialize n nsapays; flip_coins; set_announcements; compute_result]) One = One)``,
+   REPEAT STRIP_TAC
+   ++ `wp (Program [initialize n nsapays; flip_coins; set_announcements; compute_result]) One =
+       wp (Program [initialize n nsapays; flip_coins; set_announcements]) (wp compute_result One)`
+	by METIS_TAC [Program_def, wp_def, seq_assoc]
+   ++ ASM_REWRITE_TAC []
+   ++ POP_ASSUM (K ALL_TAC)
+   ++ Suff `wp compute_result One = One`
+   >> METIS_TAC [set_announcements_term]
+   ++ RW_TAC posreal_ss [compute_result_def, wp_def, One_def]);
+
+(* ???????????????????????????????????????????????
+
+val compute_result_result = store_thm
+  ("compute_result_result",
+   ``!n nsapays.
+	if nsapays
+	then
+	   wp (Program [initialize n nsapays; flip_coins; set_announcements; compute_result])
+	      (\s. if (s "result") = No then 1 else 0) = One
+	else
+	   wp (Program [initialize n nsapays; flip_coins; set_announcements; compute_result])
+	      (\s. if (s "result") = Yes then 1 else 0) = One``,
    ????);
-*)
+
+??????????????????????????????????????????????? *)
+
+(* ----------------------------- dc_prog proofs ---------------------------- *)
+
+val dcprog_term = store_thm
+  ("dcprog_term",
+   ``!n nsapays. (n > 0) ==>
+	(wp (dcprog n nsapays) One = One)``,
+   METIS_TAC [dcprog_def, compute_result_term]);
+
+(* ???????????????????????????????????????????????
+
+val dcprog_result = store_thm
+  ("dcprog_result",
+   ``!n nsapays f f'.
+	(n > 1) ==>
+	   if nsapays
+	   then
+		wp (dcprog n nsapays) (\s. if (s "result") = No then 1 else 0) = One
+	   else
+		(wp (dcprog n nsapays) (\s. if (s "result") = Yes then 1 else 0) = One) /\
+		(Leq (wp (dcprog n nsapays)
+			 (\s. if ~(i = (s "payer"))
+			      then
+				(if (f (s "N") (s "Announces") (s "result")) = (s "payer") 
+				 then 1 else 0)
+			      else
+				0))
+		     (\s. if ~ (i = (s "payer")) then (1/n) else 0)) /\
+		(Leq (wp (dcprog n nsapays)
+			 (\s. if ~(i = (s "payer"))
+			      then
+				(if i = 0
+				 then
+				    (if (f (s "N") (s "Announces") (s "result")
+					   (get_Array_i (s "Coins") 0)
+					   (get_Array_i (s "Coins") (n-1))) =
+					(s "payer")
+				     then 1 else 0)
+				 else
+				    (if (f (s "N") (s "Announces") (s "result")
+					   (get_Array_i (s "Coins") i)
+					   (get_Array_i (s "Coins") (i-1))) =
+					(s "payer")
+				     then 1 else 0))
+			      else 0))
+		     (\s. if ~(i = (s "payer")) then (1/(n-1)) else 0))``,
+   ??????);
+
+??????????????????????????????????????????????? *)
 
 val _ = export_theory();
